  \subsection{4} 
  \begin{enumerate}
    \item[a)] 12.43(5) \\
      $u_{tt}=2\Delta u$ \\
      $u|_{t=0}=2x^{2}-y^{2}, \ u_{t}|_{t=0}=2x^{2}+y^{2}$
      \begin{gather*}
        u = v + w \\
        \begin{cases}
          v_{tt} = 2 \Delta v \\ v|_{t=0} = 2x^{2} \\ v_{t}|_{t=0}=2x^{2}
        \end{cases} \begin{cases}
          w_{tt}=2\Delta w \\ w|_{t=0}=-y^{2} \\ w_{t}|_{t=0}=y^{2}
        \end{cases} \\
        v = v|_{t=0}+tv_{t}|_{t=0}+ \frac{t^{2}}{2}v_{tt}|_{t=0} + \frac{t^{3}}{6}v_{ttt}|_{t=0} + \ldots \\
        v_{tt}|_{t=0}= 2\Delta v|_{t=0}=2\Delta(v|_{t=0}) = 8 \\
        v_{ttt}|_{t=0}=2\Delta v_{t}|_{t=0}=8 \\
        v = 2x^{2}+2tx^{2}+4t^{2} + \frac{4}{3}t^{3}\\
        w = w|_{t=0}+tw_{t}|_{t=0}+ \frac{t^{2}}{2}w_{tt}|_{t=0} + \frac{t^{3}}{6}w_{ttt}|_{t=0} + \ldots \\
        w_{tt}|_{t=0}= 2\Delta w|_{t=0}=2\Delta(w|_{t=0}) = -4 \\
        w_{ttt}|_{t=0}=2\Delta w_{t}|_{t=0}=4 \\
        w = -y^{2}+ty^{2}-2t^{2} + \frac{2}{3}t^{3} \\
        \boxed{u = 2x^{2}-y^{2}+(2x^{2}+y^{2})t+2t^{2}+2t^{3}}
      \end{gather*} \newpage
      12.44(7) \\
      $u_{tt}=a^{2}\Delta u + \cos x \sin y e^{z}$ \\
      $u|_{t=0}=x^{2}e^{y+z}, \ u_{t}|_{t=0}= \sin x e^{y+z}$ \\
      \begin{gather*}
        u = v + w \\
        \begin{cases}
          v_{tt}=a^{2}\Delta v + \cos x \sin y e^{z} \\
          v|_{t=0}=0 \\
          v_{t}|_{t=0} = \sin x e^{y+z} \\
        \end{cases} \begin{cases}
          w_{tt} = a^{2}\Delta w \\
          w|_{t=0}=x^{2}e^{y+z} \\
          w_{t}|_{t=0} = 0\\
        \end{cases} \\
          v = h_{1}(t)\cos x \sin y e^{z} + h_{2}(t)\sin x e^{y+z} \\
          \begin{split}
            h_{1}'' \cos x \sin y e^{z} + h_{2}'' \sin x e^{y+z} &= a^{2}(-h_{1}\cos x \sin y e^{z} +
            h_{2} \sin x e^{y+z}) \ + \\  &+ \cos x \sin y e^{z} \\
          \end{split} \\
          \begin{cases}
            h_{1}'' = -a^{2} h_{1} + 1 \\ h_{2}'' = a^{2}h_{2}
          \end{cases} \\
          h_{1} = A \cos (at) + B \sin (at) + \frac{1}{a^{2}} \\
          h_{2} = C \sh (at) + D \ch(at) \\
          h_{1}|_{t=0} = h_{2}|_{t=0} = 0 \Rightarrow D = 0, \: A = - \frac{1}{a^{2}} \\
          h_{1_{t}}|_{t=0} = 0 \Rightarrow B = 0 \qquad h_{2_{t}}|_{t=0} = 1 \Rightarrow C = \frac{1}{a} \\
          h_{1 } =  \frac{1}{a^{2}} (1 - \cos (at)) \qquad
          h_{2} = \frac{1}{a}\sh(at) \\
          v = \frac{1}{a^{2}} (1 - \cos (at)) \cos x \sin y e^{z} + \frac{1}{a}\sh(at) \sin x e^{y+z} \\
          w = h_{3}(t)x^{2}e^{y+z}+h_{4}(t)e^{y+z} \\
          h_{3}''x^{2}e^{y+z}+h_{4}''e^{y+z} = a^{2}(h_{3}(2e^{y+z}+2x^{2}e^{y+z})+2h_{4}e^{y+z}) \\
          \begin{cases}
            h_{3}''=2a^{2}h_{3} \\ h_{4}''=2a^{2}h_{3}+2a^{2}h_{4} \\
          \end{cases} \\
      \end{gather*} \newpage
      \begin{gather*}
          h_{3} = A \ch(\sqrt{2}at) + B \sh(\sqrt{2}at) \\
          h_{3}|_{t=0} = 1 \Rightarrow A = 1 \qquad h_{3_{t}}|_{t=0} = 0 \Rightarrow B = 0 \\
          h_{3} = \ch(\sqrt{2}at) \\
          h_{4}'' -2a^{2}h_{4}=2a^{2}\ch(\sqrt{2}at) \\
          h_{4_\text{общ}} = C\ch(\sqrt{2}at)+D\sh(\sqrt{2}at) \\
          h_{4_{\text{частн}}} = t(E\ch(\sqrt{2}at)+F\sh(\sqrt{2}at)) \\
          \begin{split}
            2a^{2}t(E\ch(\sqrt{2}at)+F\sh(\sqrt{2}at)) &+\sqrt{2}a(E\ch(\sqrt{2}at)+F\sh(\sqrt{2}at) ) - \\ 
                                                       &- 2a^{2}t(E\ch(\sqrt{2}at)+F\sh(\sqrt{2}at)) =\\
                                                       &= 2a^{2}\ch(\sqrt{2}at) \\
          \end{split} \\
          E = 0, \: F = \frac{a}{\sqrt{2}} \\
          h_{4} = \frac{a}{\sqrt{2}}t\sh(\sqrt{2}at) + C\ch(\sqrt{2}at)+D\sh(\sqrt{2}at) \\
          h_{4}|_{t=0}=0 \Rightarrow C = 0 \qquad h_{4_{t}}|_{t=0} = 0 \Rightarrow D = 0 \\
          h_{4}= \frac{at}{\sqrt{2}}\sh(\sqrt{2}at) \\
          w = \ch(\sqrt{2}at)x^{2}e^{y+z}+ \frac{at}{\sqrt{2}}\sh(\sqrt{2}at)e^{y+z} \\
          \boxed{
          \begin{split}
            u = \frac{1}{a^{2}}(1-\cos(at))e^{z}\cos x \sin y &+ e^{y+z} \times \left[ \frac{1}{a}\sh(at)\sin x\right. \\ 
                                                              &+ \left.\frac{at}{\sqrt{2}}\sh(at \sqrt{2})+x^{2}\ch(at \sqrt{2})\right]
        \end{split}}
      \end{gather*} \\
      \newpage
    \item[\text{б)}] 
      $u_{tt}=\Delta u + (x^{2}+y^{2})\sin t , \: t > 0$ \\
      $u|_{t=0}=0, \: u_{t}|_{t=0}= (x^{2}+y^{2}+z^{2})^{5 / 2} - y^{2}$ \\
      \begin{gather*}
        u = v + w + p \\
        1)
          \begin{cases}
            v_{tt} = \Delta v + (x^{2}+y^{2})\sin t \\
            v|_{t=0}=0 \\ v_{t}|_{t=0} = 0
          \end{cases} 2) \begin{cases}
            w_{tt} = \Delta w \\ w|_{t=0}=0 \\ w_{t}|_{t=0}=-y^{2} \\
          \end{cases} \\
          3) \begin{cases}
            p_{tt} = \Delta p \\ p|_{t=0} = 0 \\ p_{t}|_{t=0} = (x^{2}+y^{2}+z^{2})^{5 / 2} 
          \end{cases} \\
          1) v = h_{1}(t)(x^{2}+y^{2}) + h_{2}(t) \\
          h_{1}''(x^{2}+y^{2})+h_{2}''=4h_{1}+(x^{2}+y^{2})\sin t \\
          \begin{cases}
            h_{1}'' = \sin t \\ h_{2}''=4h_{1} \\
          \end{cases} \begin{cases}
            h_{1}=-\sin t + At + B \\ 
            h_{1}|_{t=0} = 0 \\ h_{1_{t}}|_{t=0} = 0 \\
          \end{cases} \Rightarrow B = 0, \quad A = 1 \\
          \begin{cases}
            h_{1} = t - \sin t \\ h_{2}'' = 4t - 4\sin t \\
          \end{cases} \begin{cases}
            h_{2}= \frac{2}{3}t^{3}+4\sin t +Ct + D \\ h_{2}|_{t=0} = 0 \\
            h_{2_{t}}|_{t=0} = 0
          \end{cases} \Rightarrow D = 0 \quad C = -4 \\
          h_{2}= \frac{2}{3}t^{3}+4\sin t - 4t \\
        2) w = w_{t}|_{t=0} + tw_{t}|_{t=0} + \frac{t^{2}}{2}w_{tt}|_{t=0}+ \frac{t^{3}}{6}w_{ttt}|_{t=0} + \ldots \\ 
        w_{ttt}|_{t=0} = \Delta (w_{t}|_{t=0}) = -2 \\
        w =  -ty^{2} - \frac{t^{3}}{3} \\
        \end{gather*} \newpage
        \begin{gather*}
        3) x^{2}+y^{2}+z^{2} = r^{2} \\
        \begin{cases}
          p_{tt} = p_{r r} + \frac{2}{r}p \\ p|_{t=0}= 0 \\ p_{t}|_{t=0}=r^{5} \\
        \end{cases} \\
        p = \frac{s}{r} \\
        \begin{cases}
          s_{tt} = s_{r r} \\ s|_{t=0} = 0 \\ s_{t}|_{t=0} = r^{6} \\ s|_{r=0} = 0
        \end{cases} \\
        s = f(r+t) + g(r-t) \\
        \begin{cases}
          s|_{t=0} = f(r)+g(r)= 0 \\ s_{t}|_{t=0} = f'(r)-g'(r)=r^{6} \\
        \end{cases} \begin{cases}
          f(r) = \frac{r^{7}}{14}+C \\ g(r) = - \frac{r^{7}}{14} - C
        \end{cases} \\
        s = \frac{(r+t)^{7}-(r-t)^{7}}{14} \\
        p = \frac{s}{r} = \frac{(\sqrt{x^{2}+y^{2}+z^{2}}+t)^{7}-(\sqrt{x^{2}+y^{2}+z^{2}}-t)^{7}}{14 \sqrt{x^{2}+y^{2}+z^{2}}} \\
        \boxed{u = v + w + p}
      \end{gather*} \newpage
    \item[\text{в)}] $\begin{cases}
        u_{tt}=8 \Delta u +x \\ u|_{t=0}= e^{y-z} \\ u_{t}|_{t=0}=x^{2}+ y^{2}+z^{2}
      \end{cases}$
      \begin{gather*}
        u = v + w+p \\
        1) \begin{cases}
          v_{tt}=8 \Delta v+x \\ v|_{t=0}=0 \\ v_{t}|_{t=0}=0
        \end{cases} \qquad v = h(t)x, \quad h''x = x \\
        \begin{cases}
          h''=1 \\ h(0) = 0 \\ h'(0)
        \end{cases} \Rightarrow
        h(t) = \frac{t^{2}}{2}+At+B \quad v = \frac{t^{2}}{2}x \\
        2) \begin{cases}
          w_{tt} = 8 \Delta w \\ w|_{t=0}= e^{y-z} \\ w_{t}|_{t=0}=0
        \end{cases} \qquad w = h(t)e^{y-z} \\
        \begin{cases}
          h''e^{y-z}=16he^{y-z} \\ h(0) = 1 \\ h'(0) = 0
        \end{cases}\qquad h'' = 16h \Rightarrow h = A\sh(4t) + B\ch(4t) \\
        h(0) = B = 1 \quad h'(0) = 4A = 0 \Rightarrow w = \ch(4t)e^{y-z}\\
        3) \begin{cases}
          p_{tt}=0 \\ p|_{t=0}=0 \\ p_{t}|_{t=0}=x^{2}+y^{2}+z^{2} 
        \end{cases}\qquad p = t \cdot \underbrace{p_{t}|_{t=0}}_{x^{2}+y^{2}+z^{2}}+ \frac{t^{2}}{2}p_{tt}|_{t=0} +\ldots \\
        p_{tt}|_{t=0}=8\Delta (p|_{t=0})=0 \\
        p_{ttt}|_{t=0}=8 \Delta( p_{t}|_{t=0}) = 8 \Delta (x^{2}+y^{2}+z^{2}) = 48 \\
        p = t(x^{2}+y^{2}+z^{2})+ 48\frac{t^{3}}{6} \\
        \boxed{u = t(x^{2}+y^{2}+z^{2})+8t^{3}+\ch(4t)e^{y-z}+ \frac{xt^{2}}{2}}
      \end{gather*}  \newpage
    \item[\text{г)}] $u_{tt}=\Delta u -81(t+1)^{2}\sh (2x-2y+z)$ \\
      $u|_{t=0}=(2x+y-z)\cos y; \ u_{t}|_{t=0}=x^{2}-y^{2}+z^{2}$\\
      \begin{gather*}
        / \text{Fun facts...} \\
        \Delta (\sh (2x-2z+z))=9 \sh (2x-2x+z) \\
        \begin{split}
          \Delta ((2x+y-z)\cos y) &= \frac{\partial}{\partial y}(\cos y -(2x+y-z)\sin y) \\
                                  &=-2\sin y - (2x+y-z)\cos y \\
        \end{split} \\
        \Delta (x^{2}-y^{2}+z^{2})=2=0 \cdot (x^{2}-y^{2}+z^{2})+2\cdot 1 \\
        / \text{now, solution} \\
        u = v + w \\
         1) \begin{cases}
             v_{tt}=\Delta v - 81(t+1)^{2}\sh (2x-2y+z) \\ v|_{t=0}=0 \\ v_{t}|_{t=0} = 0 \\
          \end{cases} \\
          v = h(t)\sh(2x-2y+z) \\
          h''=\sh(2x-2z+z)=h\cdot 9 \sh)2x-2y+z)-81(t+1)^{2}\sh(2x-2y+z) \\
          h''=9h-81(t+1)^{2} \\
          \begin{cases}
            h''=9h-81(t+1)^{2} \\ h(0)=0 \\ h'(0)=0
          \end{cases} \\
          h = A\sh(3t)+B\ch(3t) \\
          h_{\text{частн}} = \alpha t^{2}+\beta t +\gamma \\
          2\alpha = 9\alpha t^{2}+9\beta t +9\gamma - 81t^{2}-162t-81 \\
          \begin{array}{l}
            \alpha = 9 \\ \beta = 18 \\ \gamma = 11
          \end{array} \\
          \end{gather*}
          \begin{gather*}
          h = A \sh(3t) +B\ch(3t)+9t^{2}+18t+11 \\
          h(0)=B+11=0 \rightarrow B = -11 \\
          h'(0) = 3A + 18 =0 \rightarrow A = -6 \\
          \boxed{v=(-6\sh(3t)-11\ch(3t)+9t^{2}+18t+11)\sh(2x-2y+z)} \\
        2) \begin{cases}
          w_{tt}= \Delta w \\ w|_{t=0}=(2x+y-z)\cos y \\ w_{t}|_{t=0}=0 
        \end{cases} \\
        w = h_{1}(t)(2x+y-z)\cos y + h_{2}(t)\sin y \\
        h''(2x+y-z)\cos y + h_{2}''\sin y = h_{1}(-2\sin y - (2x+y-z)\cos y)+h_{2}(-\sin y) \\
        \begin{cases}
          h_{1}''=-h_{1} \\ h_{1}(0) = 1 \\ h_{1}'=0
        \end{cases}
        \begin{cases}
          h_{2}''=-2h_{1}-h_{2} \\ h_{2}(0) = 0 \\ h_{2}'(0) = 0
        \end{cases} \\
        h_{1}=A\cos{t}+B\sin{t} \quad h_{1}(0) = A = 1, \quad h_{1}'(0)=B=0 \\
        h_{1}(t)=\cos{t} \\
        h_{2}''=-2\cos{t}-h_{2} \quad h_{2,\text{частн}}=\alpha t \cos{t}+\beta t \sin{t} \\
        h_{2,\text{частн}}'=\alpha \cos{t} -\alpha t\sin{t}+\beta \sin{t}+\beta t \cos{t} \\
        -2\alpha \sin{t}-\alpha t \cos{t} +2\beta \cos{t}-\beta t \sin{t} = -2\cos{t}-\alpha t \cos{t} - \beta t \sin{t} \\
        \begin{array}{l}
          \alpha = 0 \\ \beta = -1
        \end{array} \\
        \boxed{w=\cos{t}(2x+y-z)\cos{y}-t\sin{t}\sin{y}} \\
      3) \begin{cases}
          p_{tt}=\Delta p \\ p|_{t=0}=0 \\ p_{t}|_{2=0}=x^{2}-y^{2}+z^{2}
        \end{cases} \\
        p = h_{1}(t)(x^{2}-y^{2}+z^{2})+h_{2}(t) \\
        h''_{1}(x^{2}-y^{2}+z^{2})+h_{2}''=2h_{1} \\
        \end{gather*}
        \begin{gather*}
        \begin{cases}
          h_{1}''=0, \\ h_{1}(0) = 0, \\ h_{1}'(0)=1;
        \end{cases} \quad
        \begin{cases}
          h_{2}''=2h_{1}, \\ h_{2}(0)=0, \\ h_{2}'(0)=0;
        \end{cases} \\
        h_{1}=At+B \: \Rightarrow \: h_{1}=t \\
        h_{2}= \frac{t^{3}}{3}+At+B \: \Rightarrow \: h_{2}= \frac{t^{3}}{3}+At \\
        \boxed{p = t(x^{2}-y^{2}+z^{2})+ \frac{t^{3}}{3}} \\
        \boxed{\begin{split}
            u &= t(x^{2}-y^{2}+z^{2})+ \frac{t^{3}}{3} +\cos{t}(2x+y-z)\cos{y}-t\sin{t}\sin{y} + \\ 
              &+ (-6\sh(3t)-11\ch(3t)+9t^{2}+18t+11)\sh(2x-2y+z)
    \end{split}}
  \end{gather*} \newpage
      \item[\text{д)}] 
        $u_{tt}= \frac{1}{5}\Delta u +2t^{2}\cos(x+2y)$ \\
        $u|_{t=0}=yz^{3}, \ u_{t}|_{t=0}= \frac{1}{1+(x-2z)^{2}}$ \\
    \end{enumerate}
    \begin{gather*}
      u = v + w + p \\
      1) \begin{cases}
        v_{tt}= \frac{1}{5}\Delta v +2t^{2}\cos(x+2y) \\ v|_{t=0}=0 \\ v_{t}|_{t=0} = 0
      \end{cases} \\
      v = h(t)\cos(x+2y) \\
      h''\cos(x+2y) = \frac{1}{5}h(-5)\cos(x+2y)+2t^{2}\cos(x+2y) \\
      \begin{cases}
        h''=-h+2t^{2} \\ h(0) = 0 \\ h'(0) = 0
      \end{cases} \\
      h_{\text{частн}} = \alpha t^{2}+\beta t+\gamma \\
      2\alpha = -\alpha t^{2}-\beta t -\gamma +2t^{2} \\
      \begin{array}{l}
        \alpha = 2 \\ \beta = 0 \\ \gamma = -4
      \end{array} \\
      h = -2t^{2}-4+a\sin{t}+B\cos{t} \\
      h(0)=-4+B=0 \rightarrow B = 4 \\
      h'(0)=A=0 \\
      h(t)=2t^{2}-4+4\cos{t} \\
      v = \cos(x+2y)(2t^{2}-4+4\cos t) \\
      \end{gather*} \newpage
      \begin{gather*}
      2) \begin{cases}
        w_{tt}= \frac{1}{5}\Delta w \\ w|_{t=0}=yz^{3} \\ w_{t}|_{t=0}=0
      \end{cases} \\
      w =  \underbrace{w|_{t=0}}_{yz^{3}}+t \underbrace{w_{t}|_{t=0}}_{0}+ \frac{t^{2}}{2}w_{tt}|_{t=0} + \ldots \\
      w_{tt}= \frac{1}{5}\Delta(w|_{t=0})= \frac{1}{5}\Delta(yz^{3}) = \frac{6}{5}yz \\
      w = yz^{3}+ \frac{t^{2}}{2} \frac{6}{5}yz \\
      \end{gather*}
      \begin{gather*}
      3) \begin{cases}
        p_{tt}= \frac{1}{5}\Delta p \\ p|_{t=0}=0 \\ p_{t}|_{t=0}= \frac{1}{1+(x-2z)^{2}}
      \end{cases} \\
      x - 2z = \xi \\
      p = p(t, x-2z) = p(t, \xi)\\
      \begin{cases}
        p_{tt}= \frac{1}{5}p_{\xi \xi}\cdot 5 = p_{\xi \xi} \\
        p|_{t=0}=0 \\ p_{t}|_{t=0}= \frac{1}{1+\xi^{2}}
      \end{cases} \\
      p = \frac{1}{2}\int_{\xi-t}^{\xi+t} \frac{1}{1+\mu^{2}} \,d\mu = \frac{1}{2}(\arctg(\xi+t)-\arctg(\xi - t)) \\
      \boxed{\begin{split}
          u &= \frac{1}{2}\left(\arctg(x-2z+t)-\arctg(x-2z-t)\right)+yz^{3}+ \frac{3t^{2}}{5}yz + \\
            &+\cos(x+2y)(2t^{2}-4+4\cos t)
      \end{split}}
    \end{gather*}
  \end{enumerate} \newpage
  % \item[T1] $u_{t}= \frac{1}{4}\Delta u +t^{4}(x+1)$ \\
  %   $u|_{t=0}=e^{2z-z^{2}}\sin(x+y)$ \\
  %   \begin{gather*}
  %     u = v + w(t,z) \cdot p (t,x,y) \\
  %     1) \begin{cases}
  %       v_{t}= \frac{1}{4}\Delta v +t^{4}(x+1) \\
  %       v_{t=0}=0 \\
  %     \end{cases} \\
  %     v = h(t)(x+1) \\
  %     h'(x+1)= \frac{1}{4} h \cdot 0 +t^{4}(x+1) \\
  %     \begin{cases}
  %       h'=t^{4} \\ h(0) = 0
  %     \end{cases} \\
  %     h = \frac{t^{5}}{5} \\
  %     2) \begin{cases}
  %       w_{t}= \frac{1}{4}\Delta w \\ w|_{t=0}=e^{2z-z^{2}}
  %     \end{cases} \\
  %     w(t,z) = \frac{1}{\sqrt{\pi t}}\int_{-\infty}^{\infty} e^{- \frac{(\xi-z)^{2}}{t}}e^{2\xi-\xi^{2}} \,d\xi \\
  %     - \frac{\xi^{2}}{t}+2 \frac{z\xi}{t}- \frac{z^{2}}{t}+2\xi-\xi^{2}=-\xi^{2}( \frac{1}{t}+1)
  %     +\xi- \frac{z^{2}}{t} = \\
  %     -\left[(\xi \sqrt{ \frac{1}{t}+1})^{2}-2\xi \sqrt{ \frac{1}{t}+1}\cdot \frac{\frac{z}{t}+1}{ \sqrt{ \frac{1}{t}+1}}+ \frac{(\frac{z}{t}+1)^{2}}{ \frac{1}{t}+1}\right]
  %     + \frac{(z+t)^{2}}{t(t+1)} - \frac{z^{2}}{t} = -(\xi \sqrt{ \frac{1}{t}+1}- \frac{z+t}{\sqrt{t(t+1)}})^{2}+ \frac{z^{2}+2zt+t^{2}-tz^{2}-z^{2}}{t(t+1)} \\
  %     w = \frac{e^{\frac{2z-z^{2}+t}{t+1}}}{\sqrt{\pi t}}\int_{-\infty}^{\infty} e^{-\xi \sqrt{\frac{1}{t}+1}-\frac{z+t}{\sqrt{t(t+1)}}} \,d\xi=
  %     =\frac{1}{\sqrt{1+ \frac{1}{t}}}\int_{-\infty}^{\infty} e^{-\xi^{2}} \,d\xi = e^{\frac{2z-z^{2}+t}{\sqrt{t+1}}} \\
  %     3) \begin{cases}
  %       p_{t=0}= \frac{1}{4}\Delta p \\ p|_{t=0}=\sin(x+y) 
  %     \end{cases} \\
  %   \end{gather*}
  % \item[\text{б)}] \[
  %   \begin{cases}
  %   u_{tt}= \Delta u +(x^{2}+y^{2})\sin{t} \\ u|_{t=0}=0, \ u_{t}|_{t=0}=(x^{2}+y^{2}+z^{2})^{5 /2}-y^{2}
  % \end{cases}
  % \]
  %   \begin{gather*}
  %     u = v+w+p \\
  %     1) \begin{cases}
  %       v_{tt}= \Delta v + (x^{2}+y^{2}
  %     \end{cases}
  %   \end{gather*}
  % \item[Т4]
  %   \begin{enumerate}
  % \item[T5] $\Delta u = 4 \frac{(x-y)^{2}}{(x^{2)+y^{2}})^{3}}$
  %   \begin{gather*}
  %     u_{r r} + \frac{1}{2}u_{r}+ \frac{1}{r^{2}}u_{\varphi \varphi}= 4 \frac{(\cos\varphi-\sin\varphi)^{2}}{r^{4}= \frac{4}{r^{4}}} - \frac{4\sin(2\varphi)}{r^{4}} \\
  %     \Delta v = 0 \\
  %     v_{r}|_{r=1}= 2\sin \varphi \cos \varphi - \sin 2 \varphi = 2 \\
  %     \begin{split}
  %     (v_{r}+v)|_{r=2} &= \frac{1}{8} (\sin^{2} \varphi + \cos^{2} \varphi +2\sin \varphi \cos \varphi) + \frac{1}{4} + \frac{1}{4}\ln 2 \varphi \\ 
  %                      &- \frac{1}{8} \sin 2 \varphi - \frac{1}{4}  -\frac{1}{4}\ln 2 \sin 2 \varphi = \frac{1}{8} \\
  %     \end{split} \\
  %     v = A + B \ln r \\
  %     v_{r}|_{r=1}=B=2 \\
  %     (v_{2}+v)|_{r=2}= \frac{B}{2}+A+B\ln 2 = \frac{1}{8} \\
  %     u = \frac{1}{2}r + \frac{1}{r^{2}}\ln r \sin 2 \varphi + (- \frac{7}{8}-2 \ln 2)+2 \ln r \\
  %   \end{gather*} \\
  % \item[T6]   При каком $\alpha$ $\Delta u = y, \: r < 2$ \\
  %   $u_{r}|_{r=2} = \sin^{3} \varphi + \alpha \cos^{2} \varphi$ имеет решение? И найти это решение \\
  %   \begin{gather*}
  %     \int_{r=2}(\sin^{3} \varphi + \alpha \cos^{2} \varphi  )\,ds = \int_{0}^{2 \pi}
  %     (\sin^{3} \varphi + \alpha \cos^{2} \varphi )\,2d \varphi = \\
  %     2 \int_{0}^{2\pi} (1-\cos^{3} \varphi)\sin \varphi \,d \varphi = \alpha \int_{0}^{2\pi} (1+\cos 2 \varphi) \,d \varphi = \\
  %     2\left.\left[(-\cos \varphi + \frac{\cos^{3} \varphi}{3})\right] \right|_{0}^{2\pi}+
  %     \alpha(\varphi + \frac{\sin 2 \varphi}{2})|_{0}^{2\pi} = 2\alpha \pi \\
  %     u_{r r} + \frac{1}{r}u_{r}+ \frac{1}{r^{2}}u_{\varphi \varphi} = r \sin \varphi \\
  %     u_{\text{частн}} = \alpha r^{3} \sin \varphi \\
  %     6 \alpha r \sin \varphi + 3 \alpha r \sin \varphi - \alpha r \sin \varphi = 2 \sin \varphi \\
  %     8 \alpha = 1 \Rightarrow \alpha = \frac{1}{8} \\
  %     u = \frac{1}{8}r^{3} \sin \varphi + v \\
  %     \begin{cases}
  %       \Delta v = 0 \\ v_{r}|_{r=2}=\sin 3 \varphi - \frac{3}{2}\sin \varphi = - \frac{3}{4}\sin \varphi - \frac{1}{4} \sin 3 \varphi 
  %     \end{cases} \\
  %     v = Ar \sin \varphi + Br^{3}\sin 3 \varphi \\
  %     v_{r}|_{r=2}= A \sin \varphi + 12 B \sin 3 \varphi = - \frac{3}{4}\sin \varphi - \frac{1}{4}\sin 3 \varphi \\
  %     A = - \frac{3}{4} \quad B = - \frac{1}{48} \\
  %   \end{gather*}
  % \end{enumerate}
