\subsection{5}
$u_{tt}= a^{2}\Delta u, \ t > 0, \ x = (x_{1},x_{2},x_{3})\in \mathbb{R}^{3}$ \\
$u_{0}(x) \in C^{3}(\mathbb{R}^{3}), \ u_{1}(x)\in C^{2}(\mathbb{R}^{3}), \ r = \sqrt{x^{2}+y^{2}+z^{2}}$ \\
\begin{gather*}
  \begin{cases}
    u_{tt} = a^{2}(u_{r r}+ \frac{2}{r}u_{r}) \\ u|_{t=0}=\alpha(r) \\ u_{t}|_{t=0}= \beta(r) \\
  \end{cases} \\
  u = \frac{v}{r} \\
  u_{r}= \frac{v_{r}}{r} - \frac{v}{r^{2}} \qquad v_{r r} = \frac{v_{r r}}{r} - \frac{2v_{r}}{r^{2}} + \frac{2v}{r^{3}} \\
  \frac{v_{tt}}{r} = a^{2}( \frac{v_{r r}}{r} - \frac{2v_{r}}{r^{2}} + \frac{2v}{r^{3}}+\frac{2v_{r}}{r^{2}} - \frac{2v}{r^{3}}) = \frac{a^{2}v_{rr}}{r}\\
  \begin{cases}
    \frac{v_{tt}}{r} = \frac{a^{2}v_{rr}}{r} \\ \frac{v|_{t=0}}{r} = \alpha(r) \\ \frac{v|_{t=0}}{r} = \beta(r) \\
    \end{cases} \begin{cases}
    v_{tt} = a^{2}v_{r r} \\ v|_{t=0} = \alpha(r)r \\ v_{t}|_{t=0} = \beta(r)r \\
  \end{cases} \\
  v = \alpha\frac{(r+at)^{2}-(r-at)^{2}}{2} + \frac{1}{2a} \int_{r -at}^{r +at} \beta(R)R \,dR \\
\end{gather*} \\
\subsection{6} 
$4u_{tt}= \Delta u, \: t > 0, \: (x,y,z) \in \mathbb{R}^{3}$ \\
$u|_{t=0} = 0, \: u_{t}|_{t=0}= \begin{cases}
  \ln(1+x^{2}+y^{2}+z^{2}), \ &(x,y,z) \in G, \\ 0. &(x,y,z) \in \mathbb{R}^{3} \setminus G,
\end{cases}$ 
\begin{gather*}
  u(\vec{x},t) = \frac{1}{\pi t}  \iint_{S}^{} u_{t}|_{t=0}(\vec y) \,dS_{y}
  + \frac{\partial}{\partial t} \frac{1}{\pi t} \iint_{S}^{}u|_{t=0}(\vec y)  \,dS_{y} = \\
  = \frac{1}{\pi t} \iint_{\left|\vec x - \vec y \right| = \frac{t}{2}}^{} u_{t}|_{t=0}(\vec y)  \,dS_{y}+ \frac{1}{\pi} \frac{\partial}{\partial t} \frac{1}{t} \iint_{\left|\vec x - \vec y \right| = \frac{t}{2}}^{}  u|_{t=0}(\vec y)\,dS_{y} \\
  \vec x = \vec 0 \\
  u(\vec 0, t) =  \frac{1}{\pi t} \iint_{\left| \vec y \right| = \frac{t}{2}}^{} u_{t}|_{t=0}(\vec y)  \,dS_{y}+ \frac{1}{\pi} \frac{\partial}{\partial t} \frac{1}{t} \underbrace{\iint_{\left| \vec y \right| = \frac{t}{2}}^{}  u|_{t=0}(\vec y)\,dS_{y}}_{0} = \\
  = \frac{1}{\pi t} \iint_{\left| \vec y \right| = \frac{t}{2}}^{} \ln(1 + (\vec y)^{2})  \,dS_{y}   
  = \frac{1}{\pi t}\ln(1 + \frac{t^{2}}{4}) \iint_{\left| \vec y \right| = \frac{t}{2}}^{}   \,dS_{y}  = \\
  = \frac{1}{\pi t}\ln(1 + \frac{t^{2}}{4}) \frac{4\pi |\vec y|^{2}}{4} = 
  \frac{1}{\pi t}\ln(1 + \frac{t^{2}}{4}) \frac{\pi t^{2}}{4} = \frac{t}{4} \ln(1 + \frac{t^{2}}{4}) \\
\end{gather*} \newpage
