\subsection{1}
\begin{enumerate}
  \item[a)]  
    $u_{t}= \Delta u + e^{-9t}\cos(2x-y+2z), \ t>0, \ (x,y,z) \in \mathbb{R}^{3}$ \\
    $u|_{t=0}=xy^{2}z^{3}+\cos y \sin (x+y+z), \ (x,y,z) \in \mathbb{R}^{3}$ \\
    \begin{gather*}
      u = v + w \\
      1) \begin{cases}
        v_{t}= \Delta v \\ v|_{t=0} = xy^{2}z^{3} 
        \end{cases} 2)\begin{cases}
        w_{t} = \Delta w+ e^{-9t}\cos (2x-y+2z) \\ w|_{t=0} = 0
      \end{cases} \\
      \Delta v_{t}|_{t=0} = 2xz^{3} + 6xy^{2}z \qquad \Delta v_{tt}|_{t=0} = 24xz\\
      1)v = v|_{t=0}+tv_{t}|_{t=0}+ \frac{t^{2}}{2}v_{tt}|_{t=0} = xy^{2}z^{3} + t(2xz^{3}+6xy^{2}z)+
      12t^{2}xz \\
      2)w=h(t)\cos (2x-y+2z) \\
      h'\cos (2x-y+2z)=h(-9\cos (2x-y+2z))+e^{-9t}\cos(2x-y+2z) \\
      h'+9h=e^{-9t} \\
      h_{\text{частн}} = Ae^{-9t}t \: \Rightarrow \: A = 1 \\
      h = Ce^{-9t}+te^{-9t} \: h(0) = 0 \Rightarrow C = 0 \\
      w = te^{-9t}\cos(2x-y+2z) \\
      \boxed{u = te^{-9t}\cos(2x-y+2z)+xy^{2}z^{3} + t(2xz^{3}+6xy^{2}z)+
      12t^{2}xz }
    \end{gather*} \newpage
  \item[\text{б)}] $u_{t}= \frac{1}{4}\Delta u + t^{4}(x+1), \: t>0, \: (x,y,z) \in \mathbb{R}^{3}$ \\
    $u|_{t=0}=e^{2z-z^{3}}\sin(x+y), \: (x,y,z) \in \mathbb{R}^{3}$ \\
    \begin{gather*}
      u = v+ w \\
      1) \begin{cases}
        v_{t} = \frac{1}{4}\Delta v + t^{4}(x+1) \\ v|_{t=0} = 0\\
        \end{cases} \quad 2) \begin{cases}
        w_{t=0} = \frac{1}{4}\Delta w \\ w|_{t=0} = e^{2z-z^{3}}\sin(x+y) \\
      \end{cases} \\
      1) v = h(t) (x+1) \\
      h'(x+1) = t^{4}(x+1) \Rightarrow h' = t^{4} \\
      h= \frac{t^{5}}{5} + C \\
      h(0) = 0 \Rightarrow  C = 0 \\
      v = \frac{t^{5}}{5}(x+1) \\
      2) w = p(z,t)q(x,y,t) \\
      \begin{cases}
        p_{t} = \frac{1}{4}\Delta p \\ p|_{t=0} = e^{2z - z^{2}} \\
        \end{cases} \qquad \begin{cases}
        q_{t}= \frac{1}{4}\Delta q \\ q|_{t=0} = \sin(x+y) \\
      \end{cases} \\
      q = f(t)\sin(x+y) \\
      f'\sin(x+y) = - \frac{f}{2}\sin(x+y) \Rightarrow f'+ \frac{1}{2}f = 0 \\
      f = Ce^{-t /2} \quad f(0) = 1 \Rightarrow C = 1 \\
      q = e^{-t /2}\sin(x+y) \\
      p(t,z) = \frac{1}{\sqrt{\pi t}}\int_{-\infty}^{+\infty} e^{-(\xi - z)^{2} /t} \cdot e^{2\xi - \xi^{2}} \,d\xi = \\
      = \frac{1}{\sqrt{\pi t}}\int_{-\infty}^{+\infty} \exp(- \frac{\xi^{2}}{t} +
      \frac{2z\xi}{t} - \frac{z^{2}}{t} + 2\xi - \xi^{2}) \,d\xi = \\
      = \frac{1}{\sqrt{\pi t}}\int_{-\infty}^{+\infty} \exp(-\xi^{2}
      ( \frac{1}{t}+1)+2\xi(1+ \frac{z}{t})- \frac{z^{2}}{t}) \,d\xi = \\
    \end{gather*} \newpage
    \begin{gather*}
      = \frac{1}{\sqrt{\pi t}}\int_{-\infty}^{+\infty} \exp\left(-\left
      (\xi \sqrt{\frac{1}{t}+1} - \frac{t+z}{\sqrt{t(t+1)}}\right)^{2}
    + \frac{(t+z)^{2}}{t(t+1)}- \frac{z^{2}}{t}\right) \,d\xi = \\
    = \frac{e^{(-z^{2}+t+2z) /(t+1)}}{\sqrt{\pi t}}\int_{-\infty}^{+\infty} \sqrt{ \frac{t}{1+t}}e^{-\mu^{2}} \,d\mu = \\
    = \frac{e^{(-z^{2}+t+2z) /(t+1)}}{\sqrt{\pi t}} \sqrt{ \frac{t}{1+t}} \sqrt{\pi} =\frac{e^{(-z^{2}+t+2z) /(t+1)}}{\sqrt{t+1}} \\
    \boxed{u = \frac{e^{(-z^{2}+t+2z) /(t+1)}e^{- t /2}}{\sqrt{t+1}}+\frac{t^{5}}{5}(x+1) }
  \end{gather*} \\
\item[\text{в)}] $u_{t}= \Delta u + x^{2}y^{2}\sin t, \: t>0 , \: (x,y,z) \in \mathbb{R}^{3}$ \\
  $u|_{t=0}=xyz\cos x$ \\
  \begin{gather*}
    u = v + w \\
    1)\begin{cases}
      v_{t} = \Delta v + x^{2}y^{2}\sin t \\ v|_{t=0} = 0
      \end{cases} \qquad 2) \begin{cases}
      w_{t} = \Delta w \\ w|_{t=0} = xyz\cos x 
    \end{cases} \\
    1) v = h_{1}x^{2}y^{2} + (x^{2}+y^{2})h_{2}(t) + h_{3}(t) \\
    x^{2}y^{2}h_{1}' + (x^{2}+y^{2})h_{2}'+h_{3}' = 2(x^{2}+y^{2})h_{1}+4h_{2}+x^{2}y^{2}\sin t \\
    \begin{cases}
      h_{1}' = \sin t \\ h_{2}' = 2h_{1} \\ h_{3}' = 4h_{2} 
    \end{cases} \\
    h_{1} = -\cos t + C \quad h(0) = 0 \Rightarrow C = 1 \\
    h_{1} = 1 - \cos t \\
    h_{2} = 2t - 2\sin t + C \quad h_{2}(0) = 0 \Rightarrow C = 0 \\
    h_{3} = 4t^{2} +8\cos t + C \quad h_{3}(0) = 0 \Rightarrow C = -8 \\
  \end{gather*} \newpage
  \begin{gather*}
    v = x^{2}y^{2}(1-\cos t) + (x^{2}+y^{2})2(t-\sin t) +4t^{2}+8\cos t - 8 \\
    2)w=p(x,t)q(y,z,t) \\
    \begin{cases}
      p_{t} = \Delta p \\ p|_{t=0} = x\cos x
      \end{cases} \qquad \begin{cases}
      q_{t} = \Delta q \\ q|_{t=0} = yz 
    \end{cases} \\
    q = q|_{t=0}+tq_{t}|_{t=0} = yz \\
    p = h_{1}(t)x\cos x + h_{2}(t)\sin x \\
    h_{1}'(t)x\cos x +h_{2}'\sin x = h_{1}(-x\cos x -2\sin x) - h_{2}\sin x \\
    \begin{cases}
      h_{1}'(t) = -h_{1} \\ h_{2}'(t) = -2h_{1}-h_{2} \\
    \end{cases} \\
    h_{1} = Ce^{-t} \quad h_{1}(0) = 1 \Rightarrow C = 1 \\
    h_{1} = e^{-t} \\
    h_{2}' = -2e^{-t} - h_{2} \: \Rightarrow \: h_{2} = Ae^{-t} - 2te^{-t} \\
    h_{2}(0) = 0 \Rightarrow A = 0 \\
    h_{2} = -2te^{-t} \\
    \boxed{
      \begin{split}
        u &= (-2te^{-t}\sin x + e^{-t}x\cos x)yz +x^{2}y^{2}(1-\cos t) \ + \\
          &+(x^{2}+y^{2})2(t-\sin t) +4t^{2}+8\cos t - 8
    \end{split}}
  \end{gather*} \newpage
\item[\text{г)}] 13.5(5) \\
  $u_{t}=u_{xx}+\sin t$ \\
  $u|_{t=0}=e^{-x^{2}}$ \\
  \begin{gather*}
    u = v + w \\
    1) \begin{cases}
      v_{t} = v_{xx} + \sin t \\ v|_{t=0} = 0 
      \end{cases} \qquad 2) \begin{cases}
      w_{t} = w_{xx} \\ w|_{t=0} = e^{-x^{2}}
    \end{cases} \\
    1) v = h(t) \quad h'(t) = \sin t \quad h = -\cos t + C \\
    h(0) = 0 \Rightarrow C = 1 \quad h = 1 - \cos t \\
    v = 1 - \cos t \\
    2) w = \frac{1}{\sqrt{4 \pi t}} \int_{-\infty}^{+\infty} e^{-(\xi - x)^{2} / 4t}e^{-\xi^{2}} \,d\xi = \\
    = \frac{1}{2 \sqrt{\pi t}} \int_{-\infty}^{+\infty} \exp\left(- \frac{\xi^{2}}{4t} 
    - \frac{x^{2}}{4t}+ \frac{x\xi}{2t}-\xi^{2}\right) \,d\xi = \\
    = \frac{1}{2 \sqrt{\pi t}} \int_{-\infty}^{+\infty} \exp\left(-\left(\xi \sqrt{ \frac{4+t}{4t}}
    - \frac{x}{\sqrt{4t(4t+1)}}\right)^{2}+ \frac{x^{2}}{4t(4t+1)}- \frac{x^{2}}{4t}\right) \,d\xi = \\
    = \frac{e^{-\frac{x^{2}}{4t+1}}}{2 \sqrt{\pi t}} \int_{-\infty}^{+\infty}  \exp\left(-\left(\xi \sqrt{ \frac{4+t}{4t}}
    - \frac{x}{\sqrt{4t(4t+1)}}\right)^{2}\right)\,d\xi  = \\
    =\frac{e^{-\frac{x^{2}}{4t+1}}}{2 \sqrt{\pi t}} \int_{-\infty}^{+\infty} \sqrt{ \frac{4t}{4+t}} e^{-\mu^{2}} \,d\mu  
    = \frac{e^{-\frac{x^{2}}{4t+1}}}{2 \sqrt{\pi t}} \sqrt{ \frac{4t}{4t+1}} \sqrt{\pi} =
    \frac{e^{-\frac{x^{2}}{4t+1}}}{2 \sqrt{4t+1}} \\
    \boxed{u = 1 - \cos t + \frac{e^{-\frac{x^{2}}{4t+1}}}{2 \sqrt{4t+1}} }
  \end{gather*} \newpage
  13.5(7) \\
  $u_{t} = u_{xx}$ \\
  $u|_{t=0} = xe^{-x}$ \\
  \begin{gather*}
    u = \frac{1}{2 \sqrt{\pi t}} \int_{-\infty}^{+\infty} e^{-  \frac{(\xi -x)^{2}}{4t}}\xi
    e^{-\xi^{2}} \,d\xi = \frac{1}{2 \sqrt{\pi t}} \int_{-\infty}^{+\infty}
    \xi\exp\left(- \frac{\xi^{2}}{4t}- \frac{x^{2}}{4t} + \frac{x\xi}{2t} - \xi^{2}\right) \,d\xi = \\
    = \frac{1}{2 \sqrt{\pi t}} \int_{-\infty}^{+\infty}
    \xi\exp\left(-\left(\xi \sqrt{ \frac{4t+1}{4t}}- \frac{x}{\sqrt{4t(4t+1)}}\right)^{2}- \frac{x^{2}}
    {4t+1}\right) \,d\xi = \\
     \left/ u =\left(\xi \sqrt{ \frac{4t+1}{4t}}
    - \frac{x}{\sqrt{4t(4t+1)}}\right) \Rightarrow \xi =\sqrt{ \frac{4t+1}{4t}}\left(u 
    + \frac{x}{\sqrt{4t(4t+1)}}\right)\right / \\
    = \frac{1}{2 \sqrt{\pi t}}e^{- \frac{x^{2}}{4t+1}} \sqrt{ \frac{4t}{4t+1}}
    \int_{-\infty}^{+\infty} \sqrt{ \frac{4t}{4t+1}}\left(u 
    + \frac{x}{\sqrt{4t(4t+1)}}\right) e^{-u^{2}} \,du = \\
    = \boxed{\frac{xe^{-\frac{x^{2}}{4t+1}}}{(4t+1)^{3 /2}}}
  \end{gather*} \\
  13.6(3) \\
  $u_{t} = \Delta u + \cos t$ \\
  $u|_{t=0} = xye^{-x^{2}-y^{2}}$ \\
  \begin{gather*}
    u = v + p(x,t)q(y,t) \\
    1)\begin{cases}
      v_{t}=\Delta v + \cos t \\ v|_{t=0} = 0 
    \end{cases} \qquad 2) \begin{cases}
      p_{t} = \Delta p \\ p|_{t=0} = xe^{-x^{2}}
    \end{cases} \qquad 3) \begin{cases}
      q_{t} = \Delta q \\ q|_{t=0} = ye^{-y^{2}}
    \end{cases} \\
    v = \sin t \quad p = \frac{xe^{-\frac{x^{2}}{4t+1}}}{(4t+1)^{3 /2}} \quad 
    q = \frac{ye^{-\frac{y^{2}}{4t+1}}}{(4t+1)^{3 /2}} \\
    \boxed{u =  \sin t + \frac{xe^{-\frac{x^{2}}{4t+1}}}{(4t+1)^{3 /2}}
    + \frac{ye^{-\frac{y^{2}}{4t+1}}}{(4t+1)^{3 /2}}}
  \end{gather*}
\end{enumerate} \newpage \newpage
