\section{7}
$\delta u = 6 z, \: r < 1$ \\
$u|_{r=1} = 2\sin^{2} \varphi \sin^{2} \theta + \cos^{3} \theta$ \\
\begin{gather*}
  u_{r r} + \frac{2}{r}u_{r} + \frac{1}{r^{2}}u_{\theta \theta} + \frac{1}{r^{2}} u_{\theta} \cth 
  \theta + \frac{1}{r^{2}\sin \theta} u_{\varphi \varphi} = 6r\cos \theta \\
  u = ar^{3}\cos \theta \qquad 6ar \cos \theta + 6 a r \cos \theta - ar\cos \theta =6r\cos \theta \\
  10a = 6 \rightarrow a = 0,6 \\
  u_{\text{частн}} = 0,6r^{3}\cos \theta \\
  v = u - u_{\text{частн}} \\
  v|_{r=1} = u|_{r=1} - u_{\text{частн}}|_{r=1} = 2\sin^{2} \varphi \sin^{2} \theta + \cos^{3} \theta
  - 0,6\cos^{3} \theta = \\
  = (1-\cos 2 \varphi)\sin^{2} \theta + 0,4 \cos^{3} \theta = 0,4 \cos^{3} \theta + \sin^{2} \theta -
  \cos 2 \varphi \sin^{2} \theta = \\
  = \frac{4}{25}\underbrace{\left( \frac{5}{2} \cos^{3}\theta - \frac{3}{2}\cos \theta\right)}_{y^{*}_{3}} + \underbrace{\frac{6}{25}\cos \theta}_{y^{*}_{1}}
+ \underbrace{\frac{2}{3}}_{y^{*}_{0}} - \underbrace{\frac{2}{3}\left( \frac{3}{2}\cos^{2} \theta - \frac{1}{2}\right)}_{y^{*}_{2}} - \underbrace{\cos 2 \varphi \sin^{2} \theta }_{y^{*}_{2}}\\
  v = y_{0}+ry_{1}+r^{2}y_{2}+r^{3}y_{3} \\
  v|_{r=1} = y_{0}+y_{1}+y_{2}+y_{3}= y^{*}_{0}+y^{*}_{1}+y^{*}_{2}+y^{*}_{3} \\
  \boxed{
  \begin{split}
    u &= 0,6 r^{3} \cos \theta + \frac{2}{3} + \frac{6}{25}r\cos \theta + \frac{4}{25}\left( \frac{5}{2}\cos^{3} \theta - \frac{3}{2}\cos \theta\right)r^{3} \\
      &+r^{2}\left( - \frac{2}{3}\left( \frac{3}{2}\cos^{2} \theta - \frac{1}{2}\right) - \sin^{2}\theta \cos 2 \varphi\right) \\
\end{split}}
\end{gather*}
